\documentclass{report}

\usepackage{amsmath}
\usepackage{tcolorbox}

\renewcommand{\exp}[1]{\operatorname{exp} \left(#1\right)}
\renewcommand{\arctan}[1]{\operatorname{arctan} \left(#1\right)}

\title{Exercise 1}
\author{Daniel Gallo, Esther Jerez, Ole Kristian, Sebastian Merkesdal}

\begin{document}
    \maketitle
    
    \section*{Exercise 1}
    \begin{tcolorbox}[title=Part a]
        Find all solutions $z$ of
        \begin{equation*}
            z^3 = 4i - 4
        \end{equation*}
    \end{tcolorbox}
    \noindent
    Using polar form,
    \begin{equation*}
        z^3 = 4i - 4 = 4\sqrt{2}\exp{\frac{3\pi}{4}i}
    \end{equation*}
    We know that the principal root will have radius $r = \sqrt[3]{4\sqrt{2}}$ and argument $\theta_1 = \frac{\pi}{4}$. The other two roots will be evenly spaced throughout the circle of radius $r$. Thus,
    \begin{align*}
        \theta_1 &= \frac{\pi}{4} \\
        \theta_2 &= \theta_1 + \frac{2\pi}{3} = \frac{11\pi}{12} \\
        \theta_3 &= \theta_2 + \frac{2\pi}{3} = \frac{19\pi}{12} = \frac{-5\pi}{12} \mod{2\pi}\\
    \end{align*}
    \begin{tcolorbox}[title=Part b]
        Write the numbers below on rectangular form
        \begin{equation*}
            (\sqrt{3} - i)^{10} \quad (2 - i)^{9}
        \end{equation*}
    \end{tcolorbox}
    \begin{align*}
        (\sqrt{3} - i)^{10} &= \left(2\exp{-\frac{\pi}{6}i}\right)^{10} = 2^{10}\exp{-\frac{5\pi}{3}i} \\
        &= 2^{10}\left(\frac{1}{2} + \frac{\sqrt{3}}{2}i\right) = 512 + 512\sqrt{3}i
    \end{align*}
    \begin{equation*}
        (2 - i)^{9} = \left(\sqrt{5}\exp{\arctan{-\frac{1}{2}}i}\right)^{9} = -718 + 1199i
    \end{equation*}

    \section*{Exercise 3}
    \begin{tcolorbox}[title=Part a]
        Consider the function $w$ given by
        \begin{equation*}
            w = u + vi = \frac{1}{(iz)^2} = \frac{1}{(-y + ix)^2}
        \end{equation*}
        Find $u(x, y)$ and $v(x, y)$
    \end{tcolorbox}
    \noindent
    \begin{align*}
        w &= \frac{1}{(-y + ix)^2} = \frac{1}{y^2 - x^2 -2xyi} \\
        &= \frac{1}{y^2 - x^2 -2xyi} \frac{y^2 - x^2 + 2xyi}{y^2 - x^2 + 2xyi} \\
        &= \underbrace{\frac{y^2 - x^2}{(x^2 + y^2)^2}}_{u(x, y)} + \underbrace{\frac{2xy}{(x^2 + y^2)^2}}_{v(x, y)}i
    \end{align*}
\end{document}
